CN: Do translation validation of resource inference steps in Rocq [work in progress] (#898)
* added missing Makefile dependnecy for `cn-with-coq`

* map_from_list implemented

* Switching to MSetWeakList from FSetAVL to avoid ordering.

* Reasoning module. Proof automation sketch. Correctnes theorem generated.

* enable CI on resource-reasoning branch

* Record -> TRecord to avoid keyword name collision

* decidable equality wip

* do not export proof log in tests (to speed up)

* defining res. inf. simple case constraints

* Ltac2 automation for resource inference

* more ltac2 automation

* Switching to FSet from MSet (to take advantage of Ltac2.FSet)

* admitting ResSet equality and proving submsumption

* Latc2 automation

* new ProofAutomation module

* generating theorem.

* debug messages removed

* proving set equality

* proof log unit tests enabled

* logging unfolding. unfolding correcntess predicate placeholder

* deetecting do-nothing unfolding steps

* --coq-check-proof-log command line option

* unfold_step predicate, shelving errors

* more verbose messages in automation

* formatting

* do not export mucore AST unless --coq-mucore is specified

* wip on resource unfolding predicate

* struct members bijection in resource_unfold (wip)

* incorporating `resource_unfold` into `unfold_step`

* typo fixed

* packing/unpacking reasoning wip

* Coq code reorg, added Implementation. WIP on unfolding predicates.

* indentation

* more debugging

* streamlining `struct_piece_to_resource`

backend/cn/bin/main.ml
@@ -133,7 +133,9 @@ let with_well_formedness_check
   ~incl_dirs
   ~incl_files
   ~coq_export_file
+  ~coq_mucore
   ~coq_proof_log
+  ~coq_check_proof_log
   ~csv_times
   ~log_times
   ~astprints
@@ -183,14 +185,21 @@ let with_well_formedness_check
       in
       Result.iter_error handle_error (Typing.pause_to_result paused);
       let@ _ = f ~cabs_tunit ~prog5 ~ail_prog ~statement_locs ~paused in
-      let steps = Prooflog.get_proof_log () in
       Option.iter
         (fun path ->
-          Pp.print_file
-            path
-            (Pp_mucore_coq.pp_unit_file_with_resource_inference
-               prog5
-               (if coq_proof_log then Some steps else None)))
+          let prologue = Pp_mucore_coq.pp_prologue () in
+          let mucore =
+            if coq_mucore then Pp_mucore_coq.pp_unit_file prog5 else PPrint.empty
+          in
+          let proof =
+            if coq_proof_log then (
+              let steps = Prooflog.get_proof_log () in
+              Pp_mucore_coq.pp_proof_log steps coq_check_proof_log)
+            else
+              PPrint.empty
+          in
+          let doc = PPrint.( ^^ ) prologue (PPrint.( ^^ ) mucore proof) in
+          Pp.print_file path doc)
         coq_export_file;
       return ()
     in
@@ -268,7 +277,9 @@ let well_formed
     ~incl_dirs
     ~incl_files
     ~coq_export_file:None
+    ~coq_mucore:false
     ~coq_proof_log:false
+    ~coq_check_proof_log:false
     ~csv_times
     ~log_times
     ~astprints
@@ -296,7 +307,9 @@ let verify
   diag
   lemmata
   coq_export_file
+  coq_mucore
   coq_proof_log
+  coq_check_proof_log
   only
   skip
   csv_times
@@ -349,7 +362,9 @@ let verify
     ~incl_dirs
     ~incl_files
     ~coq_export_file
+    ~coq_mucore
     ~coq_proof_log
+    ~coq_check_proof_log
     ~csv_times
     ~log_times
     ~astprints
@@ -460,7 +475,9 @@ let generate_executable_specs
     ~incl_dirs
     ~incl_files
     ~coq_export_file:None
+    ~coq_mucore:false
     ~coq_proof_log:false
+    ~coq_check_proof_log:false
     ~csv_times
     ~log_times
     ~astprints
@@ -530,7 +547,9 @@ let run_seq_tests
     ~incl_files
     ~csv_times
     ~coq_export_file:None
+    ~coq_mucore:false
     ~coq_proof_log:false
+    ~coq_check_proof_log:false
     ~log_times
     ~astprints
     ~no_inherit_loc
@@ -650,7 +669,9 @@ let run_tests
     ~incl_files
     ~csv_times
     ~coq_export_file:None
+    ~coq_mucore:false
     ~coq_proof_log:false
+    ~coq_check_proof_log:false
     ~log_times
     ~astprints
     ~no_inherit_loc
@@ -1004,14 +1025,26 @@ end
 
 module CoqExport_flags = struct
   let coq_export =
-    let doc = "export to coq" in
+    let doc = "File to export to coq defintions" in
     Arg.(value & opt (some string) None & info [ "coq-export-file" ] ~docv:"FILE" ~doc)
+end
+
+module CoqMucore_flags = struct
+  let coq_mucore =
+    let doc = "include mu-core AST in coq export" in
+    Arg.(value & flag & info [ "coq-mucore" ] ~doc)
 end
 
 module CoqProofLog_flags = struct
   let coq_proof_log =
     let doc = "include proof log in coq export" in
-    Arg.(value & flag & info [ "coq-proof-log" ] ~docv:"FILE" ~doc)
+    Arg.(value & flag & info [ "coq-proof-log" ] ~doc)
+end
+
+module CoqCheckProofLog_flags = struct
+  let coq_check_proof_log =
+    let doc = "Include statements to check proof log in coq exported file" in
+    Arg.(value & flag & info [ "coq-check-proof-log" ] ~doc)
 end
 
 let wf_cmd =
@@ -1062,7 +1095,9 @@ let verify_t : unit Term.t =
   $ Verify_flags.diag
   $ Lemma_flags.lemmata
   $ CoqExport_flags.coq_export
+  $ CoqMucore_flags.coq_mucore
   $ CoqProofLog_flags.coq_proof_log
+  $ CoqCheckProofLog_flags.coq_check_proof_log
   $ Verify_flags.only
   $ Verify_flags.skip
   $ Common_flags.csv_times
