backend/cn/coq/Cn/BaseTypes.v
@@ -1,11 +1,26 @@
-Require Import Cerberus.Symbol.
+Require Import Coq.Program.Equality.
+Require Import Coq.Structures.DecidableType.
+Require Import Coq.Structures.DecidableTypeEx.
+
+Require Import StructTact.StructTactics.
+
+Require Import Coq.Arith.Arith.
+Require Import Coq.Init.Wf.
+Require Import Coq.Arith.Wf_nat.
+Require Import Coq.Wellfounded.Inverse_Image.
+Require Import Coq.Lists.List.
+Import ListNotations.
+
+Require Import Sym.
 Require Import Id.
 
 Inductive sign : Type :=
   | Signed
   | Unsigned.
 
+Unset Elimination Schemes.
 Inductive t_gen (A:Type) : Type :=
+  (* base cases *)
   | Unit : t_gen A  
   | Bool : t_gen A
   | Integer : t_gen A
@@ -15,30 +30,238 @@ Inductive t_gen (A:Type) : Type :=
   | Alloc_id : t_gen A
   | Loc : A -> t_gen A
   | CType : t_gen A
-  | Struct : Symbol.t -> t_gen A
-  | Datatype : Symbol.t -> t_gen A
-  | Record : list (Symbol.identifier * t_gen A) -> t_gen A
+  | Struct : Sym.t -> t_gen A
+  | Datatype : Sym.t -> t_gen A
+  (* recursive cases *)
+  | TRecord : list (Symbol.identifier * t_gen A) -> t_gen A
   | Map : t_gen A -> t_gen A -> t_gen A
   | List : t_gen A -> t_gen A
   | Tuple : list (t_gen A) -> t_gen A
   | TSet : t_gen A -> t_gen A.
+Set Elimination Schemes.
+
+Inductive Forall_type {A : Type} (P : A -> Type) : list A -> Type :=
+| Forall_nil : Forall_type P nil
+| Forall_cons : forall (x : A) (xs : list A), P x -> Forall_type P xs -> Forall_type P (x :: xs).
+
+(* We define a custom induction principle for [t_gen] because the
+   default one incorrectly handles hidden recursive cases for the
+   [TFunction] and [Tuple] constructors. *)
+Theorem t_gen_ind_set (A : Type) (P : t_gen A -> Type):
+  (* base cases *)
+  P (Unit A) ->
+  P (Bool A) ->
+  P (Integer A) ->
+  P (MemByte A) ->
+  (forall (s : sign) (n : nat), P (Bits A s n)) ->
+  P (Real A) ->
+  P (Alloc_id A) ->
+  (forall a : A, P (Loc A a)) ->
+  P (CType A) ->
+  (forall t : Sym.t, P (Struct A t)) ->
+  (forall t : Sym.t, P (Datatype A t)) ->
+  (* recursive cases *)
+  (forall l : list (Symbol.identifier * t_gen A), (Forall_type (fun '(_,x) => P x) l) -> P (TRecord A l)) ->
+  (forall t : t_gen A, P t -> forall t0 : t_gen A, P t0 -> P (Map A t t0)) ->
+  (forall t : t_gen A, P t -> P (List A t)) ->
+  (forall l : list (t_gen A), (Forall_type P l) -> P (Tuple A l))  ->
+  (forall t : t_gen A, P t -> P (TSet A t))
+
+  -> forall t : t_gen A, P t.
+Proof.
+  intros HUnit HBool HInteger HMemByte HBits HReal HAlloc HLoc HCType HStruct HDatatype HTRecord HMap HList HTuple HTSet.
+  fix IH 1.
+  intros t.
+  destruct t; simpl.
+  - (* Unit *)
+    apply HUnit.
+  - (* Bool *)
+    apply HBool.
+  - (* Integer *)
+    apply HInteger.
+  - (* MemByte *)
+    apply HMemByte.
+  - (* Bits *)
+    apply HBits.
+  - (* Real *)
+    apply HReal.
+  - (* Alloc_id *)
+    apply HAlloc.
+  - (* Loc *)
+    apply HLoc.
+  - (* CType *)
+    apply HCType.
+  - (* Struct *)
+    apply HStruct.
+  - (* Datatype *)
+    apply HDatatype.
+  - (* TRecord *)
+    eapply HTRecord.
+    induction l.
+    + constructor.
+    + constructor.
+      break_let.
+      auto.
+      auto.
+  - (* Map *)
+    apply HMap; apply IH.
+  - (* List *)
+    apply HList; apply IH.
+  - (* Tuple *)
+    eapply HTuple.
+    induction l.
+    + constructor.
+    + constructor; auto.
+  - (* TSet *)
+    apply HTSet; apply IH.
+Qed.
 
 
 Definition member_types_gen (A:Type) := list (Id.t * t_gen A).
 
 Module Datatype.
   Record info (A : Type) := mk_info {
-    constrs : list Symbol.t;
+    constrs : list Sym.t;
     all_params : member_types_gen A
   }.
 
   Record constr_info (A : Type) := mk_constr_info {
     params : member_types_gen A;
-    datatype_tag : Symbol.t
+    datatype_tag : Sym.t
   }.
 End Datatype.
 
 Definition t := t_gen unit.
+
+Fact sign_eq_dec (s1 s2 : sign) : {s1 = s2} + {s1 <> s2}.
+Proof.
+  decide equality.
+Qed.
+
+(* TODO Check if needed *)
+Lemma prod_eq_dec {A B : Type}
+      (eqA : forall x y : A, {x = y} + {x <> y})
+      (eqB : forall x y : B, {x = y} + {x <> y}) :
+      forall (p1 p2 : A * B), {p1 = p2} + {p1 <> p2}.
+Proof.
+  decide equality.
+Qed.
+
+Module BasetTypes_t_as_MiniDecidableType <: MiniDecidableType.
+  Definition t := t.
+  Definition eq := @eq t.
+  
+  Lemma eq_dec : forall (x y : t), { eq x y } + { ~ eq x y }.
+  Proof.
+    unfold eq, t, BaseTypes.t.
+    intros x.
+    apply (t_gen_ind_set unit (fun t => forall y, { t = y } + { t <> y })).
+
+    (* fragile: assuming `y` *)
+    all: intros; destruct y; try (left; reflexivity); try (right; intros; discriminate).
+    -
+      destruct (sign_eq_dec s s0), (OrderedTypeEx.Nat_as_OT.eq_dec n n0);subst.
+      + auto.
+      + right. intros H. inversion H. contradiction.
+      + right. intros H. inversion H. contradiction.
+      + right. intros H. inversion H. contradiction.
+    -
+      destruct a, u.
+      left.
+      reflexivity.
+    -
+      destruct (Sym_t_as_MiniDecidableType.eq_dec t0 t1);
+        unfold Sym_t_as_MiniDecidableType.eq in *; subst.
+      + left; reflexivity.
+      + right. intros H. inversion H. congruence.
+    -
+      destruct (Sym_t_as_MiniDecidableType.eq_dec t0 t1);
+        unfold Sym_t_as_MiniDecidableType.eq in *; subst.
+      + left; reflexivity.
+      + right. intros H. inversion H. congruence.
+    -
+      (* TODO: this is not provavle with current induction principle! *)
+      admit.
+    -
+      specialize (H y1).
+      specialize (H0 y2).
+      inversion H.
+      +
+        subst.
+        inversion H0.
+        *
+          subst.
+          left.
+          reflexivity.
+        *
+          right.
+          intros H3.
+          inversion H3.
+          congruence.
+      +
+        right.
+        intros H3.
+        inversion H3.
+        auto.
+    -
+      specialize (H y).
+      inversion H.
+      +
+        subst.
+        left.
+        reflexivity.
+      +
+        right.
+        intros C.
+        inversion C.
+        congruence.
+    -
+      clear x.
+      revert l0.
+      induction H;intros.
+      +
+        destruct l0.
+        * left. reflexivity.
+        * right. congruence.
+      +
+        destruct l0.
+        * right. congruence.
+        * specialize (p t0).
+          specialize (IHForall_type l0).
+          f_equal.
+          inversion p.
+          --
+            subst.
+            inversion IHForall_type.
+            ++
+              inversion H0.
+              subst.
+              left.
+              reflexivity.
+            ++
+              right.
+              intros C.
+              inversion C.
+              subst.
+              congruence.
+          --
+            right.
+            intros C.
+            inversion C.
+            congruence.
+    -
+      specialize (H y).
+      destruct H.
+      + subst. left. reflexivity.
+      +
+        right.
+        intros C.
+        inversion C.
+        congruence.
+  Admitted.
+  
+End BasetTypes_t_as_MiniDecidableType.
+
 
 Definition dt_info := Datatype.info unit.
 Definition constr_info := Datatype.constr_info unit.
