backend/cn/coq/Cn/IndexTerms.v
@@ -1,7 +1,10 @@
 Require Import List.
+Require Import Coq.Structures.DecidableType.
+Require Import Coq.Structures.DecidableTypeEx.
 
 Require Import BaseTypes.
 Require Import Terms.
+Require Import Locations.
 
 (* Type aliases *)
 Definition t' := term BaseTypes.t.
@@ -10,3 +13,22 @@ Definition t := annot BaseTypes.t.
 (* Pattern-related types *)
 Definition bindings (bt: Type) := list (pattern bt * option (annot bt)).
 Definition t_bindings := bindings BaseTypes.t. 
+
+Module IndexTerm_as_MiniDecidableType <: MiniDecidableType.
+  Definition t := t.
+  Definition eq := @eq t.
+  Lemma eq_dec : forall (x y : t), { eq x y } + { ~ eq x y }.
+  Proof.
+    unfold eq.
+    decide equality; subst.
+    -
+      repeat decide equality.
+    -
+      apply BasetTypes_t_as_MiniDecidableType.eq_dec.
+    -
+      admit.
+  Admitted.
+End IndexTerm_as_MiniDecidableType. 
+
+Module IndexTerm_as_DecidableType := Make_UDT IndexTerm_as_MiniDecidableType.
+
