backend/cn/coq/Cn/Resource.v
@@ -1,3 +1,8 @@
+Require Import Coq.Structures.DecidableType.
+Require Import Coq.Structures.DecidableTypeEx.
+Require Import Coq.FSets.FSetWeakList.
+Require Import Coq.FSets.FSetDecide.
+
 Require Import Request.
 Require Import IndexTerms.
 
@@ -9,3 +14,25 @@ Definition qpredicate : Type := Request.QPredicate.t * output.
 
 Definition t : Type := Request.t * output.
 
+Module Resource_as_MiniDecidableType <: MiniDecidableType.
+  Definition t := t.
+  Definition eq := @eq t.
+  Lemma eq_dec : forall (x y : t), { eq x y } + { ~ eq x y }.
+  Proof.
+    unfold eq.
+    decide equality.
+    -
+      subst.
+      decide equality.
+      apply IndexTerm_as_MiniDecidableType.eq_dec.
+    -
+      admit.
+  Admitted.
+End Resource_as_MiniDecidableType.
+
+Module Resource_as_DecidableType := Make_UDT Resource_as_MiniDecidableType.
+Module ResSet := FSetWeakList.Make Resource_as_DecidableType.
+Module ResSetDecide := FSetDecide.WDecide(ResSet).
+
+Definition set_from_list (l : list t) : ResSet.t :=
+  List.fold_left (fun s c => ResSet.add c s) l ResSet.empty.
