backend/cn/coq/Cn/CNImpl.v
@@ -1,0 +1,183 @@
+
+Require Import Coq.Numbers.BinNums.
+Require Import Coq.Strings.String.
+Require Import Coq.ZArith.ZArith.
+Require Import Lia.
+
+Require Import AltBinNotations.
+
+Require Import StructTact.StructTactics.
+
+From Cerberus Require Import Implementation IntegerType Ctype Symbol.
+
+Local Open Scope nat_scope.
+
+Module CNImpl : Implementation.
+
+  Definition is_signed_ity_impl ity :=
+    match ity with
+    | Char => true
+    | Bool => false
+    | Signed _ => true
+    | Unsigned _ => false
+    | Enum tag_sym => true (* TODO: we do not handle registered enums *)
+    | Size_t =>  false
+    | Wchar_t => true
+    | Wint_t =>  true
+    | Ptrdiff_t => true
+    | Ptraddr_t => false
+    end.
+
+  Definition sizeof_ity_impl x
+    :=  match x with
+        | Char
+        | Bool => Some 1
+        | Signed ibty
+        | Unsigned ibty =>
+          Some (match ibty with
+            | Ichar => 1
+            | Short => 2
+            | Int_ => 4
+            | Long
+            | LongLong => 8
+            | IntN_t n
+            | Int_leastN_t n
+            | Int_fastN_t n => max 1 (Nat.div n 8)
+            | Intmax_t
+            | Intptr_t => 8
+            end)
+        | Enum ident => Some 4 (* TODO: we do not handle registered enums *)
+        | Wchar_t
+        | Wint_t => Some 4
+        | Size_t
+        | Ptrdiff_t => Some 8
+        | Ptraddr_t => Some 8
+        end.
+
+  Definition precision_ity_impl ity : option Z :=
+    match sizeof_ity_impl ity with
+    | Some n =>
+        let zn := Z.of_nat n in
+        if is_signed_ity_impl ity then
+          Some (8*zn-1)%Z
+        else
+          Some (8*zn)%Z
+    | None =>
+        None
+    end.
+
+  Definition sizeof_fty_impl x
+    := match x with
+       | RealFloating Float =>
+           Some 8 (* TODO:hack ==> 4 *)
+       | RealFloating Double =>
+           Some 8
+       | RealFloating LongDouble =>
+           Some 8 (* TODO:hack ==> 16 *)
+       end.
+
+  Definition alignof_fty_impl x : nat
+    := match x with
+       | RealFloating Float =>
+           8 (* TODO:hack ==> 4 *)
+       | RealFloating Double =>
+           8
+       | RealFloating LongDouble =>
+           8 (* TODO:hack ==> 16 *)
+       end.
+
+  Definition alignof_ity_impl x : nat :=
+    match x with
+    | Char
+    | Bool => 1
+    | Signed ibty
+    | Unsigned ibty =>
+        (match ibty with
+         | Ichar => 1
+         | Short => 2
+         | Int_ => 4
+         | Long
+         | LongLong => 8
+         | IntN_t n
+         | Int_leastN_t n
+         | Int_fastN_t n => max 1 (Nat.div n 8)
+         | Intmax_t
+         | Intptr_t => 8
+         end)
+    | Enum ident => 4 (* TODO: we do not handle registered enums *)
+    | Wchar_t
+    | Wint_t => 4
+    | Size_t
+    | Ptrdiff_t => 8
+    | Ptraddr_t => 8
+    end.
+
+  (* fixing enum type for simplicity. *)
+  Definition typeof_enum_impl (_:Symbol.sym)
+             := Signed Int_.
+
+  Program Definition get :=
+    {|
+      name            := "clang11_aarch64-unknown-freebsd13";
+      details         := "clang version 11.0.0\nTarget: Morello";
+      sizeof_pointer  := 8;
+      alignof_pointer := 8;
+      is_signed_ity   := is_signed_ity_impl;
+      sizeof_ity      := sizeof_ity_impl;
+      precision_ity   := precision_ity_impl;
+      sizeof_fty      := sizeof_fty_impl;
+      alignof_ity     := alignof_ity_impl;
+      alignof_fty     := alignof_fty_impl;
+      typeof_enum     := typeof_enum_impl;
+    |}.
+
+  Lemma ichar_size:  (sizeof_ity get (IntegerType.Signed IntegerType.Ichar) = Some 1).
+  Proof. reflexivity. Qed.
+
+  Lemma uchar_size:  (sizeof_ity get (IntegerType.Unsigned IntegerType.Ichar) = Some 1).
+  Proof. reflexivity. Qed.
+
+  Lemma alignof_pointer_pos: 0 < (alignof_pointer get).
+  Proof.
+    cbn.
+    lia.
+  Qed.
+
+  Lemma alignof_ity_pos: forall ty, 0< (alignof_ity get ty).
+  Proof.
+    intros ty.
+    destruct ty; cbn;try lia.
+    1,2: destruct i; cbn;try lia.
+
+    all: pose proof (Nat.divmod_spec n 7 0 7) as DM;
+      assert(7<=7) as SV by lia;
+      specialize (DM SV);
+      remember (Nat.divmod n 7 0 7) as dm;
+      destruct dm;
+      cbn;
+      destruct DM;
+      destruct n0;lia.
+  Qed.
+
+  Lemma alignof_fty_pos: forall ty, 0< (alignof_fty get ty).
+  Proof.
+    intros ty.
+    destruct ty; cbn;try lia.
+    destruct r; lia.
+  Qed.
+
+  Lemma sizeof_ity_pos: forall ty x, sizeof_ity get ty = Some x -> 0 < x.
+  Proof.
+    intros ty x H.
+    destruct ty;
+      cbn in H; repeat break_match_hyp; inversion H; lia.
+  Qed.
+
+  Lemma sizeof_fty_pos: forall ty x, sizeof_fty get ty = Some x -> 0 < x.
+  Proof.
+    intros ty x H.
+    destruct ty;
+      cbn in H; repeat break_match_hyp; inversion H; lia.
+  Qed.
+
+End CNImpl.
