backend/cn/coq/Cn/Terms.v
@@ -6,6 +6,7 @@ Require Import Cerberus.Symbol.
 Require Import BaseTypes.
 Require Import Cerberus.Location.
 Require Import SCtypes.
+Require Import Locations.
 Require Import Cerberus.IntegerType.
 
 (* Constants *)
@@ -74,7 +75,7 @@ Inductive pattern_ (bt : Type) : Type :=
   | PConstructor : sym -> list (Symbol.identifier * pattern bt) -> pattern_ bt
 
 with pattern (bt : Type) : Type :=
-  | Pat : pattern_ bt -> bt -> Location_t -> pattern bt.
+  | Pat : pattern_ bt -> bt -> Locations.t -> pattern bt.
 
 (* Terms *)
 Inductive term (bt : Type) : Type :=
@@ -89,7 +90,7 @@ Inductive term (bt : Type) : Type :=
   | Struct : sym -> list (Symbol.identifier * annot bt) -> term bt
   | StructMember : annot bt -> Symbol.identifier -> term bt
   | StructUpdate :  (annot bt * Symbol.identifier) -> annot bt -> term bt
-  | Record : list (Symbol.identifier * annot bt) -> term bt
+  | TRecord : list (Symbol.identifier * annot bt) -> term bt
   | RecordMember : annot bt -> Symbol.identifier -> term bt
   | RecordUpdate :  (annot bt * Symbol.identifier) -> annot bt -> term bt
   | Constructor : sym -> list (Symbol.identifier * annot bt) -> term bt
@@ -119,4 +120,4 @@ Inductive term (bt : Type) : Type :=
   | Cast : BaseTypes.t -> annot bt -> term bt
 
 with annot (bt : Type) : Type :=
-  | IT : term bt -> bt -> Location_t -> annot bt. 
+  | IT : term bt -> bt -> Locations.t -> annot bt.
