backend/cn/coq/Reasoning/ResourceInference.v
@@ -1,0 +1,308 @@
+Require Import Coq.Lists.List.
+Require Import Coq.ZArith.ZArith.
+Require Import Coq.FSets.FSetInterface.
+
+From Cerberus Require Import IntegerType Ctype.
+From Cn Require Import Prooflog Request Resource Context Sym IndexTerms BaseTypes SCtypes.
+
+Import ListNotations.
+
+(* Helper functoin to get a set of resources from the contex *)
+
+Definition ctx_resources_set (l:((list (Resource.t * Z)) * Z)) : ResSet.t
+  :=
+  Resource.set_from_list (List.map fst (fst l)).
+
+(* Relation between Sctypes.t and BaseTypes.t *)
+Inductive bt_of_sct_rel : SCtypes.t -> BaseTypes.t -> Prop :=
+| bt_of_sct_void : bt_of_sct_rel SCtypes.Void (BaseTypes.Unit unit)
+| bt_of_sct_integer : forall ity,
+    bt_of_sct_rel (SCtypes.Integer ity) 
+      (BaseTypes.Bits _ (if Memory.is_signed_integer_type ity then BaseTypes.Signed else BaseTypes.Unsigned)
+                      (Memory.sizeof_ity ity * 8))
+| bt_of_sct_array : forall sct bt,
+    bt_of_sct_rel sct bt ->
+    bt_of_sct_rel (SCtypes.Array (sct, None)) 
+      (BaseTypes.Map _ 
+        (BaseTypes.Bits _ BaseTypes.Unsigned (Memory.sizeof_ity (IntegerType.Signed Intptr_t) * 8)) 
+        bt)
+| bt_of_sct_pointer : forall sct,
+    bt_of_sct_rel (SCtypes.Pointer sct) (BaseTypes.Loc unit tt)
+| bt_of_sct_struct : forall tag,
+    bt_of_sct_rel (SCtypes.Struct tag) (BaseTypes.Struct _ tag)
+(* TODO function types *).
+
+(* Helper predicate to relate struct piece to resource *)
+Inductive struct_piece_to_resource 
+  (piece: Memory.struct_piece) 
+  (iinit: init) 
+  (ipointer: IndexTerms.t) 
+  (iargs: list IndexTerms.t) 
+  (tag: Sym.t) 
+  (loc: Location.t)
+  : output -> Resource.t -> Prop :=
+| struct_piece_to_resource_intro:
+    forall pid pty field_bt fields field_it struct_loc,
+    Memory.piece_member_or_padding piece = Some (pid, pty) ->
+    let field_pointer := Terms.IT _ (Terms.MemberShift _ ipointer tag pid) (BaseTypes.Loc _ tt) loc in
+    let field_out := Resource.O field_it in
+    (* The field's type maps to its base type *)
+    bt_of_sct_rel pty field_bt ->
+    (* field_out is the IT corresponding to pid in iout's field list *)
+    List.In (pid, field_it) fields 
+    
+    ->
+
+    struct_piece_to_resource piece iinit ipointer iargs tag loc 
+      (Resource.O (Terms.IT _ (Terms.Struct _ tag fields) (BaseTypes.Struct _ tag) struct_loc))
+      (Request.P {| Predicate.name := Request.Owned pty iinit;
+                    Predicate.pointer := field_pointer; 
+                    Predicate.iargs := iargs |},
+       field_out).
+
+Inductive resource_unfold (globals:Global.t): Resource.t -> ResSet.t -> Prop :=
+(* non-struct "Owned" resources unfold to themselves *)
+| resource_unfold_nonstruct:
+    forall ipointer iargs iout iinit ity,
+    not (SCtypes.is_struct ity) ->
+
+    resource_unfold globals
+      (Request.P 
+        {| 
+          Predicate.name := Request.Owned ity iinit; 
+          Predicate.pointer := ipointer; 
+          Predicate.iargs := iargs 
+        |}, 
+        iout) 
+      (ResSet.singleton 
+        (Request.P 
+        {| 
+          Predicate.name := Request.Owned ity iinit; 
+          Predicate.pointer := ipointer; 
+          Predicate.iargs := iargs 
+        |}, 
+        iout)         
+      ) 
+
+| resource_unfold_struct:
+  forall out_res ipointer iargs iout iinit isym sdecl loc,
+
+  (* lookup struct declaration in global environment *)
+  SymMap.MapsTo isym sdecl globals.(Global.struct_decls) ->
+
+  (* Resources are related to struct pieces *)
+  (forall r, 
+    ResSet.In r out_res <->
+      exists piece, List.In piece sdecl /\
+        struct_piece_to_resource piece iinit ipointer iargs isym loc iout r) 
+  
+  ->
+
+  resource_unfold globals
+    (Request.P 
+      {| 
+        Predicate.name := Request.Owned (SCtypes.Struct isym) iinit; 
+        Predicate.pointer := ipointer; 
+        Predicate.iargs := iargs 
+      |}, 
+      iout) 
+    out_res.
+  
+(** Inductive predicate which defines correctness of resource unfolding step *)
+Inductive unfold_step : Context.t -> Context.t -> Prop :=
+| simple_unfold_step:
+    forall 
+    icomputational ilogical iresources iconstraints iglobal
+    ocomputational ological oresources oconstraints oglobal,
+    
+  (* The following parts of context are not changed *)
+    icomputational = ocomputational ->
+    iglobal = oglobal ->
+    ilogical = ological ->
+    iconstraints = oconstraints ->
+
+    let in_res := ctx_resources_set iresources in
+    let out_res := ctx_resources_set oresources in
+
+    (* The `out_res` is union of `resource_unfold` of all resources in `in_res` *)
+    (forall r', ResSet.In r' out_res <-> 
+      exists r, ResSet.In r in_res /\ exists s, 
+      resource_unfold iglobal r s /\ ResSet.In r' s
+    ) 
+    
+    ->
+
+    unfold_step
+    (* input context *)
+    {|
+      Context.computational := icomputational;
+      Context.logical := ilogical;
+      Context.resources := iresources;
+      Context.constraints := iconstraints;
+      Context.global := iglobal
+    |}
+
+    (* output context *)
+    {|
+      Context.computational := ocomputational;
+      Context.logical := ological;
+      Context.resources := oresources;
+      Context.constraints := oconstraints;
+      Context.global := oglobal
+    |}.
+  
+
+(** Inductive predicate which defines correctess of log inference step *)
+Inductive log_entry_valid : log_entry -> Prop :=
+| unfold_resources_step:
+    forall loc c c',
+    unfold_step c c' ->
+    log_entry_valid (ResourceInferenceStep c (UnfoldResources loc) c')
+
+(* simple case: non-recursive request, no packing *)
+| simple_resource_inference_step:
+  forall iname  ipointer  iargs
+    oname  opointer  oargs
+    err out lines oloc
+    icomputational ilogical iresources iconstraints iglobal
+    ocomputational ological oresources oconstraints oglobal,
+
+  (* The following parts of context are not changed *)
+  icomputational = ocomputational ->
+  iglobal = oglobal ->
+  ilogical = ological ->
+  iconstraints = oconstraints ->
+
+  let in_res := ctx_resources_set iresources in
+  let out_res := ctx_resources_set oresources in
+
+  (* alt. definition sketch:
+  let res_diff := Resource.ResSet.diff in_res out_res in
+  Resource.ResSet.cardinal res_diff = 1 /\
+  ...
+   *)
+
+  (* [out_res] is a subset of [in_res] with exactly one element [used] removed. *)
+  (exists (upred: Request.Predicate.t),
+      ResSet.Equal (Resource.ResSet.add (P upred, out) out_res) in_res /\
+      Request.subsumed iname upred.(Request.Predicate.name)
+  ) 
+  
+  (* TODO:
+  /\ iname=oname  
+  /\ ipointer=opointer
+  /\ iargs=oargs
+  *)
+  ->
+
+    log_entry_valid
+      (ResourceInferenceStep
+         (* input context *)
+         {|
+           Context.computational := icomputational;
+           Context.logical := ilogical;
+           Context.resources := iresources;
+           Context.constraints := iconstraints;
+           Context.global := iglobal
+         |}
+
+         (* request type *)
+         (PredicateRequest
+            err (* unused *)
+            (* input predicate *)
+            {| Predicate.name:=iname; Predicate.pointer:=ipointer; Predicate.iargs:=iargs |}
+            oloc (* unused *)
+            ((
+                (* output predicate *)
+                {| Predicate.name:=oname; Predicate.pointer:=opointer; Predicate.iargs:=oargs |},
+                  out
+              ), lines (* unused *)
+         ))
+
+         (* output context *)
+         {|
+           Context.computational := ocomputational;
+           Context.logical := ological;
+           Context.resources := oresources;
+           Context.constraints := oconstraints;
+           Context.global := oglobal
+         |}
+      )
+
+ (* struct case: struct resource is removed from input context *)
+| struct_resource_inference_step:
+  forall isym iinit ipointer iargs
+    oname opointer oargs
+    err out lines oloc
+    icomputational ilogical iresources iconstraints iglobal
+    ocomputational ological oresources oconstraints oglobal,
+
+  (* The following parts of context are not changed *)
+  icomputational = ocomputational ->
+  iglobal = oglobal ->
+  ilogical = ological ->
+  iconstraints = oconstraints ->
+
+  let in_res := ctx_resources_set iresources in
+  let out_res := ctx_resources_set oresources in
+
+  (* Find the struct resource and its fields *)
+  (exists (field_res: ResSet.t),
+      (* The struct unfolds to field resources *)
+      resource_unfold iglobal 
+        (Request.P {| Predicate.name := Request.Owned (SCtypes.Struct isym) iinit;
+                      Predicate.pointer := ipointer;
+                      Predicate.iargs := iargs |}, out)
+        field_res /\
+      (* Output context is input context minus all field resources *)
+      ResSet.Equal out_res (ResSet.diff in_res field_res)
+  ) ->
+
+  (* TODO:
+  /\ iname=oname  
+  /\ ipointer=opointer
+  /\ iargs=oargs
+  *)
+
+  log_entry_valid
+    (ResourceInferenceStep
+      (* input context *)
+      {|
+        Context.computational := icomputational;
+        Context.logical := ilogical;
+        Context.resources := iresources;
+        Context.constraints := iconstraints;
+        Context.global := iglobal
+      |}
+
+      (* request type *)
+      (PredicateRequest
+        err (* unused *)
+        (* input predicate *)
+        {| Predicate.name := Request.Owned (SCtypes.Struct isym) iinit;
+           Predicate.pointer := ipointer;
+           Predicate.iargs := iargs |}
+        oloc (* unused *)
+        ((
+                (* output predicate *)
+                {| Predicate.name:=oname; Predicate.pointer:=opointer; Predicate.iargs:=oargs |},
+                  out
+              ), lines (* unused *)
+         )
+      )
+
+      (* output context *)
+      {|
+        Context.computational := ocomputational;
+        Context.logical := ological;
+        Context.resources := oresources;
+        Context.constraints := oconstraints;
+        Context.global := oglobal
+      |}
+    ).
+
+
+
+(** Proof log is valid if all entries are valid *)
+Definition prooflog_valid (l:Prooflog.log) := List.Forall log_entry_valid l.
+
